Some progress

vale/code/lib/transformers/Vale.Transformers.Transform.fst
@@ -28,10 +28,28 @@ let reorder orig hint =
       result = orig;
     }
 
+#push-options "--max_fuel 2 --max_ifuel 1"
+let lemma_code_codes (c:code) (fuel:nat) (s:machine_state) :
+  Lemma
+    (ensures (machine_eval_code c fuel s == machine_eval_codes [c] fuel s)) = ()
+
+let lemma_codes_code (c:codes) (fuel:nat) (s:machine_state) :
+  Lemma
+    (ensures (machine_eval_codes c fuel s == machine_eval_code (Block c) fuel s)) = ()
+#pop-options
+
 (* See fsti *)
 let lemma_reorder orig hint transformed va_s0 va_sM va_fM =
   match Vale.Transformers.InstructionReorder.reordering_allowed [orig] [hint] with
   | Ok () -> (
-      admit ()
+      lemma_code_codes orig va_fM (state_to_S va_s0);
+      Vale.Transformers.InstructionReorder.lemma_reordering [orig] [hint] va_fM (state_to_S va_s0);
+      lemma_codes_code (Vale.Transformers.InstructionReorder.perform_reordering [orig] [hint]) va_fM (state_to_S va_s0);
+      let Some s' = machine_eval_code transformed va_fM (state_to_S va_s0) in
+      assume (same_domain va_sM s');
+      let va_sM' = state_of_S va_sM s' in
+      assume (equiv_states va_sM va_sM');
+      assume (va_ensure_total transformed va_s0 va_sM' va_fM);
+      va_sM', va_fM
     )
   | Err reason -> va_sM, va_fM
